\documentclass{article}
\usepackage{amsmath}
\usepackage{amssymb}
\usepackage{semantic}
\usepackage[margin=1in]{geometry}
\usepackage{fancyhdr}
\usepackage{enumerate}
\usepackage[shortlabels]{enumitem}
\usepackage{systeme}
\pagestyle{fancy}
\fancyhead[L]{Katkov Fedor}
\fancyhead[C]{Calculus homework 18}
\fancyhead[R]{\today}
\begin{document}
\section*{Problem 2}
\subsection*{(a)}
$$\int\left[\cos^5{(7x + 3)}\right]dx = \left[t = (7x + 3),\implies dt = 7dx\right] = \frac{1}{7}\cdot\int\left[\cos^5{t}\right]dt = \frac{1}{7}\cdot\int\left[\cos^4{t}\cdot\cos{t}\right]dt = $$
$$ = \left[U = \sin{t},\implies dU = \cos{t}dt\right] = \frac{1}{7}\cdot\int\left[(1 - U^2)^2\right]dU = \frac{1}{7}\cdot\int dU - \frac{2}{7}\cdot\int\left[U^4\right]dU + \frac{1}{7}\cdot\int\left[U^4\right]dU = $$
$$ = \frac{U}{7} - \frac{2\cdot U^3}{21} + \frac{U^5}{35} + C = \frac{\sin{(7x + 3)}}{7} - \frac{2\cdot\sin^3{(7x + 3)}}{21} + \frac{\sin^5{(7x + 3)}}{35} + C\in\mathbb{R}$$
\subsection*{(b)}
$$\int\left[\cosh^4{x}\right]dx = \int\left[\left(\frac{1 + \cosh{2x}}{2}\right)^2\right]dx = \int\left[\frac{3 + 4\cdot\cosh{2x} + \cosh{4x}}{8}\right]dx =$$
$$ = \frac{3}{8}\cdot\int dx + \frac{1}{2}\cdot\int\left[\cosh{2x}\right]dx + \frac{1}{8}\cdot\int\left[\cosh{4x}\right]dx = \frac{3}{8}\cdot x + \frac{\sinh{2x}}{4} + \frac{\sinh{4x}}{32} + C\in\mathbb{R}$$
\subsection*{(c)}
$$\int\left[\sin^4{2x}\cdot\cos^2{2x}\right]dx = \int\left[(1 - \cos^2{2x})^2\cdot\cos^2{2x}\right]dx = \int\left[\cos^2{2x} - 2\cdot\cos^4{2x} + \cos^6{2x}\right]dx$$
$$ = \int\left[\cos^2{2x}\right]dx - 2\cdot\int\left[\cos^4{2x}\right]dx + \cdot\int\left[\cos^6{2x}\right]dx = $$
$$ = \int\left[\frac{1 + \cos{4x}}{2}\right]dx - \int\left[\frac{3 + 4\cos{4x} + \cos{8x}}{8}\right]dx + \int\left[\frac{5 + 12\cos{4x} + 6\cos{8x} + \cos{12x}}{32}\right]dx = $$
$$ = -\frac{3x}{32} + \frac{\sin{4x}}{16} + \frac{\sin{8x}}{64} + \frac{\sin{12x}}{384} + C\in\mathbb{R}$$
\newpage\section*{Problem 4}
\subsection*{(a)}
$$\int\left[\frac{\cos^3{x}}{\sqrt{\sin{x}}}\right]dx = \left[t = \sin{x},\implies dt = \cos{x}dx\right] = \int\left[\frac{(1 - t^2)}{\sqrt{t}}\right]dt = \int\left[t^{-0.5}\right]dt - \int\left[t^{1.5}\right]dt = $$
$$ = \frac{t^{0.5}}{0.5} - \frac{t^{2.5}}{2.5} + C = \frac{\sin^{0.5}{x}}{0.5} - \frac{\sin^{2.5}{x}}{2.5} + C\in\mathbb{R}$$
\subsection*{(b)}
$$\int\left[\coth^3{(2x + 3)}\right]dx = \int\left[\frac{\cosh^3{(2x + 3)}}{\sinh^3{(2x + 3)}}\right]dx = \int\left[\frac{\cosh{(2x + 3)} + \cosh{(2x + 3)}\cdot\sinh^2{(2x + 3)}}{\sinh^3{(2x + 3)}}\right]dx = $$
$$ = \int\left[\frac{\cosh{(2x + 3)}}{\sinh^3{(2x + 3)}} + \frac{\cosh{(2x + 3)}}{\sinh{(2x + 3)}}\right]dx = \int\left[\frac{\cosh{(2x + 3)}}{\sinh^3{(2x + 3)}}\right]dx + \int\left[\frac{\cosh{(2x + 3)}}{\sinh{(2x + 3)}}\right]dx = $$
$$ = \left[t = \sinh{(2x + 3)},\implies dt = 2\cosh{(2x + 3)}\right] = $$
$$= \frac{1}{2}\cdot\int\left[t^{-3}\right]dt + \frac{1}{2}\cdot\int\left[\frac{1}{t}\right]dt = -\frac{1}{4t^2} + \frac{\ln{|t|}}{2} + C = -\frac{1}{4\cdot\sinh^2{(2x + 3)}} + \frac{\ln{|\sinh{(2x + 3)}|}}{2} + C\in\mathbb{R}$$
\subsection*{(c)}
$$\int\left[\cot^4{(2 - x)}\right]dx = \int\left[\left(\frac{1}{\sin^2{(2 - x)}} - 1\right)^2\right]dx = \int\left[\frac{1}{\sin^4{(2 - x)}} - \frac{1}{\sin^2{(2 - x)}} + 1\right]dx = $$
$$ = \int\left[\frac{1}{\sin^4{(2 - x)}}\right]dx - \int\left[\frac{1}{\sin^2{(2 - x)}}\right]dx + \int dx = \left[t = 2 - x,\implies dt = -dx\right] = $$
$$ = 3\cot{t} + \frac{\cot^3{t}}{3} - t + C = 3\cot{(2 - x)} + \frac{\cot^3{(2 - x)}}{3} - (2 - x) + C\in\mathbb{R}$$
\subsection*{(d)}
$$\int\left[\sin{5x}\cdot\sin{7x}\right]dx = \frac{1}{2}\int\left[\cos{2x} - \cos{7x}\right]dx = \frac{1}{2}\left(\int\left[\cos{2x}\right]dx - \int\left[\cos{12x}\right]dx\right) = \frac{\sin{2x}}{4} - \frac{\sin{12x}}{24} + C\in\mathbb{R}$$
\subsection*{(e)}
$$\int\left[\frac{\sin{x}}{1 + 5\cos{x}}\right]dx = \left[t = 1 + 5\cos{x},\implies dt = -5\sin{x}\right] = -\frac{1}{5}\cdot\int\left[\frac{1}{t}\right]dx = -\frac{\ln{|1 + 5\cos{x}|}}{5} + C\in\mathbb{R}$$
\newpage\section*{Problem 6}
\subsection*{Problem A}
$$\int\left[\frac{1}{2\sin{x} + \cos{x} + 3}\right]dx$$
Using Universal Trigonometric Substitution we get:
$$t = \tan{\frac{x}{2}}\implies\left[\sin{x} = \frac{2t}{1 + t^2};\hspace{0.1cm}\cos{x} = \frac{1 - t^2}{1 + t^2};\hspace{0.1cm}dt = \frac{2}{1 + t^2}dt\right]\implies\left[\frac{1}{2\sin{x} + \cos{x} + 3} = \frac{2(t^2 + 2t + 2)}{1 + t^2}\right]$$
$$\int\left[\frac{1}{2\sin{x} + \cos{x} + 3}\right]dx = \int\left[\frac{\frac{2}{1 + t^2}}{\frac{2(t^2 + 2t + 2)}{1 + t^2}}\right]dx = \int\left[\frac{1}{(t + 1)^2 + 1}\right]dx = \arctan{(\tan{\frac{x}{2}} + 1)} + C\in\mathbb{R}$$
\subsection*{Problem B}
$$\int\left[\frac{1}{3\sin{x} - 4\cos{x}}\right]dx$$
Using Universal Trigonometric Substitution we get:
$$t = \tan{\frac{x}{2}}\implies\left[\sin{x} = \frac{2t}{1 + t^2};\hspace{0.1cm}\cos{x} = \frac{1 - t^2}{1 + t^2};\hspace{0.1cm}dt = \frac{2}{1 + t^2}dt\right]\implies\left[\frac{1}{3\sin{x} - 4\cos{x}} = \frac{4t^2 + 6t - 4}{t^2 + 1}\right]$$
$$\int\left[\frac{1}{3\sin{x} - 4\cos{x}}\right]dx = \int\left[\frac{1}{4t^2 + 6t - 4}\right]dx = \frac{1}{2}\cdot\int\left[\frac{1}{(t + 0.75)^2 - (1.25)^2}\right]dx = \frac{2}{5}\ln{\left|\frac{\tan{\frac{x}{2}} - 0.5 }{ \tan{\frac{x}{2}} + 2 }\right|} + C\in\mathbb{R}$$
\newpage\section*{Problem 7}
\subsection*{(a)}
$$\int\left[\frac{1}{\sqrt{1 - x^2}\cdot\sqrt[7]{\arcsin{x}}}\right]dx = \left[t = \arcsin{x},\implies dt = \frac{1}{\sqrt{1 - x^2}}dx\right] = \int\left[\frac{1}{\sqrt[7]{t}}\right]dt = $$
$$ = \frac{7}{6}\cdot t^{\frac{6}{7}} + C = \frac{7}{6}\cdot (\arcsin{x})^{\frac{6}{7}} + C\in\mathbb{R}$$
\subsection*{(b)}
$$\int\left[\frac{\cos{(\log_8{(5x + 8)})}}{x}\right]dx = \left[t = \log_8{(5x + 8)},\implies dt = \frac{5}{(5x + 8)\ln{8}}dt,\implies \frac{dx}{x} = \ln{8}\cdot dt\right] = $$
$$ = \int\left[\cos{t}\cdot\ln{8}\right] dt = \ln{8}\cdot\sin{(\log_8{(5x + 8)})} + C\in\mathbb{R}$$
\subsection*{(c)}
$$\int\left[\frac{2x + 3}{\sqrt{15 - 6x - x^2}}\right]dx = \int\left[\frac{2x + 3}{\sqrt{24 - (x + 3)^2}}\right]dx = \left[t = x - 3,\implies dt = dx\right] = \int\left[\frac{2t - 3}{\sqrt{24 - t^2}}\right]dt = $$
$$ = \int\left[\frac{2t}{\sqrt{24 - t^2}}\right]dt - \int\left[\frac{3}{\sqrt{24 - t^2}}\right]dt = -2\cdot\sqrt{24 - t^2} - 3\arcsin{\left(\frac{t}{\sqrt{24}}\right)} + C = $$
$$ = -2\cdot\sqrt{24 - (x - 3)^2} - 3\arcsin{\left(\frac{x - 3}{\sqrt{24}}\right)} + C\in\mathbb{R}$$
\end{document}
